tidying examples part 1

examples/dm4all/Exn.fst
@@ -1,6 +1,8 @@
 module Exn
 
-module List = FStar.List.Tot
+(* Reasoning about programs with exceptions, but with
+ * pure WPs, in a total correctness setting. That is,
+ * raising an exception has a false precondition. *)
 
 let repr (a:Type) = either a exn
 
@@ -31,37 +33,28 @@ new_effect {
      ; interp    = interp
 }
 
-let test1 () : EXN int (fun p -> p 5 /\ p 3) = 5
-let test2 () : EXN int (fun p -> p 5 /\ p 3) = 3
-[@expect_failure]
-let test3 () : EXN int (fun p -> p 5 /\ p 3) = 4
+let raise (#a:Type) (e:exn) : EXN a (fun p -> False)  =
+  EXN?.reflect (Inr e)
 
+(* An alias for convenience *)
 effect Ex (a:Type) (pre:pure_pre) (post:pure_post' a pre) =
         EXN a (fun (p:pure_post a) -> pre /\ (forall (pure_result:a). post pure_result ==> p pure_result))
-
-effect ExTot (a:Type) = EXN a (pure_null_wp a)
-
-(* GM: Why is this forcing me to Type0? *)
-val raise : #a:Type0 -> e:exn -> EXN a (fun p -> False)
-let raise #a e = EXN?.reflect (Inr e)
-
 exception Neg
 
 let test (x:int) : EXN int (fun p -> x >= 0 /\ (forall y. p y)) =
   if x < 0 then
     raise Neg;
   x + x
-  
+
 let test' (x:int) : Ex int (requires (x >= 0)) (ensures (fun _ -> True)) =
   if x < 0 then
     raise Neg;
   x + x
 
+(* This is an expected failure, since x could be negative, and this
+ * program should not verify with a trivial precondition. *)
 [@expect_failure]
 let test'' (x:int) : Ex int (requires True) (ensures (fun _ -> True)) =
   if x < 0 then
     raise Neg;
   x + x
-
-[@expect_failure]
-let _ = assert False
