examples/dm4all/NDDemonic.fst
@@ -9,8 +9,6 @@ let return (a:Type u#a) (x:a) = [x]
 let bind (a : Type u#aa) (b : Type u#bb)
     (l : repr a) (f : a -> repr b) = List.flatten (List.map f l)
 
-(* let choose (#a : Type) (x y : a) : repr a = [x;y] *)
-
 (* Demonic interpretation *)
 let interp (#a:Type) (l : repr a) : pure_wp a =
     fun p -> forall (x:a). List.memP x l ==> p x
@@ -30,28 +28,13 @@ new_effect {
      ; bind_wp   = pure_bind_wp
 
      ; interp    = interp
-
-     (* ; choose    = choose *)
 }
 
-let test1 () : ND int (fun p -> p 5 /\ p 3) = 5
-let test2 () : ND int (fun p -> p 5 /\ p 3) = 3
-
-// Whoa! This used to succeed since the effect is marked as reifiable,
-// and Rel compares the representation types on each side for the
-// subtyping. and both are just `unit -> list a`. I changed it to check
-// the WPs via stronger-than instead of always unfolding.
-[@expect_failure]
-let test3 () : ND int (fun p -> p 5 /\ p 3) = 4
-
 assume val test_f : unit -> ND int (fun p -> p 5 /\ p 3)
-
 let l : (l:list int{forall p. p 5 /\ p 3 ==> interp l p}) = reify (test_f ())
 
 effect Nd (a:Type) (pre:pure_pre) (post:pure_post' a pre) =
         ND a (fun (p:pure_post a) -> pre /\ (forall (pure_result:a). post pure_result ==> p pure_result))
-
-effect NDTot (a:Type) = ND a (pure_null_wp a)
 
 val choose : #a:Type0 -> x:a -> y:a -> ND a (fun p -> p x /\ p y)
 let choose #a x y =
@@ -60,6 +43,9 @@ let choose #a x y =
 val fail : #a:Type0 -> unit -> ND a (fun p -> True)
 let fail #a () =
     ND?.reflect []
+
+let flip () : ND bool (fun p -> p true /\ p false) =
+    choose true false
 
 let test () : ND int (fun p -> forall (x:int). 0 <= x /\ x < 10 ==> p x) =
     let x = choose 0 1 in
@@ -78,10 +64,7 @@ let rec pick #a (l : list a) : ND a (fun p -> forall x. List.memP x l ==> p x) =
     match l with
     | [] -> fail ()
     | x::xs ->
-      // choose x (pick xs)
-      // ^ this is wrong! it will call `pick xs` before choosing and always
-      //   end up returning []
-      if choose true false
+      if flip ()
       then x
       else pick xs
 
@@ -97,11 +80,10 @@ let pyths () : ND (int & int & int) (fun p -> forall x y z. x*x + y*y == z*z ==>
   let x = pick l in
   let y = pick l in
   let z = pick l in
-  (* funny, using == here gives a terrible error message: "Could not prove-postcondition" *)
   guard (x*x + y*y = z*z);
   (x,y,z)
 
-(* Check ND.ml for the triples:
+(* Extracted code for pyths:
 
 let (pyths_norm : unit -> (Prims.int * Prims.int * Prims.int) Prims.list) =
   fun uu____1038  ->
@@ -111,10 +93,3 @@ let (pyths_norm : unit -> (Prims.int * Prims.int * Prims.int) Prims.list) =
     ((Prims.parse_int "8"), (Prims.parse_int "6"), (Prims.parse_int "10"))]
 *)
 let pyths_norm () = normalize_term (reify (pyths ()))
-
-let test_reify_1 () = assert (reify (test1 ()) ==  [5])
-let test_reify_2 () = assert (reify (test2 ()) ==  [3])
-let test_reify_3 () = assert (reify (test1 ()) =!= [4])
-
-[@expect_failure]
-let _ = assert False
