examples/dm4all/StExn.fst
@@ -1,20 +1,16 @@
 module StExn
 
-open FStar.List
-open FStar.WellFounded
-open FStar.Tactics
-
 (* Reasoning about State plus exceptions, but WPs only over
- * the stateful part. Exceptions are all failures. *)
+ * the stateful part. Exceptions are all failures, i.e.,
+ * we consider total correctness. *)
 
 type state = int
 
 let st a = state -> option (a * state)
 
-let return (a:Type) (x:a) = fun s -> Some (x, s)
+let return (a:Type) (x:a) : st a = fun s -> Some (x, s)
 
-let bind (a : Type u#aa) (b : Type u#bb)
-         (m : st a) (f : a -> st b) : st b =
+let bind (a b : Type) (m : st a) (f : a -> st b) : st b =
   fun s -> match m s with
         | Some (v, s') -> f v s'
         | None -> None
@@ -26,13 +22,10 @@ let return_wp (a:Type) (x:a) : wpty a =
   fun h p -> p x h
 
 unfold
-val bind_wp : range -> a:Type -> b:Type -> wpty a -> (a -> wpty b) -> wpty b
-
-unfold
 let bind_wp (_ : range) (a:Type) (b:Type) (w : wpty a) (kw : a -> wpty b) : wpty b =
   fun h p -> w h (fun x h' -> kw x h' (fun y h'' -> p y h''))
-  
-let rec interpretation #a (m : st a) (s0 : state) (p : post a) : Type0 =
+
+let interpretation #a (m : st a) (s0 : state) (p : post a) : Type0 =
   match m s0 with
   | Some (x, s1) -> p x s1
   | None -> False
@@ -51,9 +44,10 @@ new_effect {
      ; return_wp = return_wp
      ; bind_wp   = bind_wp
 
-     ; interp = interpretation
+     ; interp    = interpretation
 }
 
+(* Actions *)
 val get : unit -> StExn state (fun s p -> p s s)
 let get () =
   StExn?.reflect (fun s -> Some (s,s))
@@ -72,7 +66,8 @@ let test1 () : StExn int (fun s0 p -> p 42 (s0 + 5)) =
   set (y + 3);
   42
 
-[@(expect_failure [19])]
+(* This can fail, since the initial state could be < 1 *)
+[@expect_failure]
 let test2 () : StExn int (fun s0 p -> p 42 (s0 + 5)) =
   let x = get () in
   if x < 1 then raise ();
